#### Truth values and conditional expressions

```
def select_first = λfirst.λsecond.first
def select_second = λfirst.λsecond.second
def true = select_first
def false = select_second
def cond = λe1.λe2.λc.((c e1) e2)
```

### NOT

| p | ⌐p  |
| - | :-: |
| T |  F  |
| F |  T  |

```
def not = λx.(((cond false) true) x)
```

body simplification

```
(((λe1.λe2.λc.((c e1) e2) false) true) x) =>
((λe2.λc.((c false) e2) true) x) =>
(λc.((c false) true) x) => 
((x false) true)
```

gives

```
def not = λx.((x false) true)
```

¬ TRUE ≡ FALSE

```
(not true) ==
(λx.((x false) true) true) =>
((true false) true) ==
((λfirst.λsecond.first false) true) =>
(λsecond.false true) =>
false
```

¬ FALSE ≡ TRUE

```
(not false) ==
(λx.((x false) true) false) =>
((false false) true) ==
((λfirst.λsecond.second false) true) =>
(λsecond.second true) =>
true
```

### AND

| p | q | p ∧ q |
| - | - | :---: |
| F | F |   F   |
| F | T |   F   |
| T | F |   F   |
| T | T |   T   |

```
def and = λx.λy.(((cond y) false) x)
```

body simplification

```
(((λe1.λe2.λc.((c e1) e2) y) false) x) =>
((λe2.λc.((c y) e2) false) x) =>
(λc.((c y) false) x) =>
((x y) false)
```

gives

```
def and = λx.λy.((x y) false)
```

FALSE ∧ FALSE ≡ FALSE

```
((and false) false) ==
((λx.λy.((x y) false) false) false) =>
(λy.((false y) false) false) =>
((false false) false) ==
((λfirst.λsecond.second false) false) =>
(λsecond.second false) =>
false
```

FALSE ∧ TRUE ≡ FALSE

```
((and false) true) ==
((λx.λy.((x y) false) false) true) =>
(λy.((false y) false) true) =>
((false true) false) ==
((λfirst.λsecond.second true) false) =>
(λsecond.second false) =>
false
```

TRUE ∧ FALSE ≡ FALSE

```
((and true) false) ==
((λx.λy.((x y) false) true) false) =>
(λy.((true y) false) false) =>
((true false) false) ==
((λfirst.λsecond.first false) false) =>
(λsecond.false false) =>
false
```

TRUE ∧ TRUE ≡ TRUE

```
((and true) true) ==
((λx.λy.((x y) false) true) true) =>
(λy.((true y) false) true) =>
((true true) false) ==
((λfirst.λsecond.first true) false) =>
(λsecond.true false) =>
true
```

### OR

| p | q | p ∨ q |
| - | - | :---: |
| F | F |   F   |
| F | T |   T   |
| T | F |   T   |
| T | T |   T   |

```
def or = λx.λy.(((cond true) y) x)
```

body simplification

```
(((cond true) y) x) ==
(((λe1.λe2.λc.((c e1) e2) true) y) x) =>
((λe2.λc.((c true) e2) y) x) =>
(λc.((c true) y) x) =>
((x true) y)
```

gives

```
def or = λx.λy.((x true) y)
```

FALSE ∨ FALSE ≡ FALSE

```
((or false) false) ==
((λx.λy.((x true) y) false) false) =>
(λy.((false true) y) false) =>
((false true) false) ==
((λfirst.λsecond.second true) false) =>
(λsecond.second false) =>
false
```

FALSE ∨ TRUE ≡ TRUE

```
((or false) true) ==
((λx.λy.((x true) y) false) true) =>
(λy.((false true) y) true) =>
((false true) true) ==
((λfirst.λsecond.second true) true) =>
(λsecond.second true) =>
true
```

TRUE ∨ FALSE ≡ TRUE

```
((or true) false) ==
((λx.λy.((x true) y) true) false) =>
(λy.((true true) y) false) =>
((true true) false) ==
((λfirst.λsecond.first true) false) =>
(λsecond.true false) =>
true
```

TRUE ∨ TRUE ≡ TRUE

```
((or true) true) ==
((λx.λy.((x true) y) true) true) =>
(λy.((true true) y) true) =>
((true true) true) ==
((λfirst.λsecond.first true) true) =>
(λsecond.true true) =>
true
```

### Natural numbers

```
def zero = identity
def succ = λn.λs.((s false) n)
```

```
def one = (succ zero)
def two = (succ one)
def three = (succ two)
```

```
def is_zero = λn.(n select_first)
```

```
(is_zero one) ==
(λn.(n select_first) one) =>
(one select_first) ==
((succ zero) select_first) ==
((λn.λs.((s false) n) zero) select_first) =>
(λs.((s false) zero) select_first) =>
((select_first false) zero) ==
((λfirst.λsecond.first false) zero) =>
(λsecond.false zero) =>
false
```

```
(is_zero zero) ==
(λn.(n select_first) zero) =>
(zero select_first) ==
(identity select_first) ==
(λx.x select_first) =>
select_first ==
true
```

```
def pred = λn.(((cond zero) (n select_second)) (is_zero n))
```

body simplification

```
(((cond zero) (n select_second)) (is_zero n)) ==
(((λe1.λe2.λc.((c e1) e2) zero) (n select_second)) (is_zero n)) =>
((λe2.λc.((c zero) e2) (n select_second)) (is_zero n)) =>
(λc.((c zero) (n select_second)) (is_zero n)) =>
(((is_zero n) zero) (n select_second))
```

gives

```
def pred = λn.(((is_zero n) zero) (n select_second))
```

```
(pred zero) ==
(λn.(((is_zero n) zero) (n select_second)) zero) =>
(((is_zero zero) zero) (n select_second)) ==
(((λn.(n select_first) zero) zero) (n select_second)) =>
(((zero select_first) zero) (n select_second)) ==
(((λx.x select_first) zero) (n select_second)) =>
((select_first zero) (n select_second)) ==
((λfirst.λsecond.first zero) (n select_second)) =>
(λsecond.zero (n select_second)) =>
zero
```

```
(pred one) ==
(λn.(((is_zero n) zero) (n select_second)) one) =>
(((is_zero one) zero) (one select_second)) ==
(((λn.(n select_first) one) zero) (one select_second)) =>
(((one select_first) zero) (one select_second)) ==
((((succ zero) select_first) zero) (one select_second)) ==
((((λn.λs.((s false) n) zero) select_first) zero) (one select_second)) =>
(((λs.((s false) zero) select_first) zero) (one select_second)) =>
((((select_first false) zero) zero) (one select_second)) ==
((((λfirst.λsecond.first false) zero) zero) (one select_second)) =>
(((λsecond.false zero) zero) (one select_second)) =>
((false zero) (one select_second)) ==
((λfirst.λsecond.second zero) (one select_second)) =>
(λsecond.second (one select_second)) =>
(one select_second) ==
((succ zero) select_second) ==
((λn.λs.((s false) n) zero) select_second) =>
(λs.((s false) zero) select_second) =>
((select_second false) zero) ==
((λfirst.λsecond.second false) zero) =>
(λsecond.second zero) =>
zero
```

```
(pred two) ==
(λn.(((is_zero n) zero) (n select_second)) two) =>
(((is_zero two) zero) (two select_second)) ==
(((λn.(n select_first) two) zero) (two select_second)) =>
(((two select_first) zero) (two select_second)) ==
((((succ one) select_first) zero) (two select_second)) ==
((((λn.λs.((s false) n) one) select_first) zero) (two select_second)) =>
(((λs.((s false) one) select_first) zero) (two select_second)) =>
((((select_first false) one) zero) (two select_second)) ==
((((λfirst.λsecond.first false) one) zero) (two select_second)) =>
(((λsecond.false one) zero) (two select_second)) =>
((false zero) (two select_second)) ==
((λfirst.λsecond.second zero) (two select_second)) =>
(λsecond.second (two select_second)) =>
((succ one) select_second) ==
((λn.λs.((s false) n) one) select_second) =>
(λs.((s false) one) select_second) =>
((select_second false) one) ==
((λfirst.λsecond.second false) one) =>
(λsecond.second one) =>
one
```

### λ calculus simplified notations

```
(((<function> <arg1>) <arg2>) ... <argN>) ==
<function> <arg1> <arg2> <argN>
```

```
def <names> = λ<name>.<expression> == 
def <names> name = <expression>
```

```
cond <true choise> <false choise> <cond expr> ==
if <cond expr>
then <true choise>
else <false choise>
```

#### 3.1: Implication (conditional)

| p | q | p → q |
| - | - | :---: |
| F | F |   T   |
| F | T |   T   |
| T | F |   F   |
| T | T |   T   |

```
def implies = λp.λq.(((cond q) true) p)
```

body simplification

```
(((cond q) true) p) ==
(((e1.λe2.λc.((c e1) e2) q) true) p) =>
((λe2.λc.((c q) e2) true) p) =>
(λc.((c q) true) p) =>
((p q) true)
```

gives

```
def implies = λp.λq.((p q) true)
```

simplified notations

```
def implies p q = p q true
```

FALSE → FALSE ≡ TRUE

```
implies false false => ...
false false true => ...
true
```

FALSE → TRUE ≡ TRUE

```
implies false true => ...
false true true => ...
true
```

TRUE → FALSE ≡ FALSE

```
implies true false => ...
true false true => ...
false
```

TRUE → TRUE ≡ TRUE

```
implies true true => ...
true true true => ...
true
```

#### 3.2: Equivalence (biconditional)

| p | q | p ↔ q |
| - | - | :---: |
| F | F |   T   |
| F | T |   F   |
| T | F |   F   |
| T | T |   T   |

```
def equiv = λp.λq.(((cond q) (not q)) p)
```

body simplification

```
(((cond q) (not q)) p) ==
(((λe1.λe2.λc.((c e1) e2) q) (not q)) p) =>
((λe2.λc.((c q) e2) (not q)) p) =>
(λc.((c q) (not q)) p) =>
((p q) (not q))
```

gives

```
def equiv = λp.λq.((p q) (not q))
```

simplified notations

```
def equiv p q = p q (not q)
```

FALSE ↔ FALSE ≡ TRUE

```
equiv false false => ...
fale false (not false) => ...
(not false) => ...
true
```

FALSE ↔ TRUE ≡ FALSE

```
equiv false true => ...
false true (not true) => ...
(not true) => ...
false
```

FALSE ↔ TRUE ≡ FALSE

```
equiv true false => ...
true false (not false) => ...
false
```

TRUE ↔ TRUE ≡ TRUE

```
equiv true true => ...
true true (not true) => ...
true
```

#### 3.3: show that functions are equivalent for all boolean values

##### (a) ¬p ⋀ ¬q ≡ ¬(p ⋁ q)

¬FALSE ⋀ ¬FALSE ≡ TRUE

```
λx.λy(and (not x) (not y)) false false => ...
and (not false) (not false) => ...
(not false) (not false) false => ...
true (not false) false => ...
not false => ...
true
```

¬FALSE ⋀ ¬TRUE ≡ FALSE

```
λx.λy(and (not x) (not y)) false true => ...
and (not false) (not true) => ...
(not false) (not true) false => ...
true (not true) false => ...
not true => ...
false
```

¬TRUE ⋀ ¬FALSE ≡ FALSE

```
λx.λy(and (not x) (not y)) true false => ...
and (not true) (not false) => ...
(not true) (not false) false => ...
false (not false) false => ..
false
```

¬TRUE ⋀ ¬TRUE ≡ FALSE

```
λx.λy(and (not x) (not y)) true true => ...
and (not true) (not true) => ...
(not true) (not true) false => ...
false (not true) false => ...
false
```

¬(FALSE ⋁ FALSE) ≡ TRUE

```
λx.λy(not (or x y)) false false => ...
not (or false false) => ...
(or false false) false true => ...
(false true false) false true => ...
false false true => ...
true
```

¬(FALSE ⋁ TRUE) ≡ FALSE

```
λx.λy(not (or x y)) false true => ...
not (or false true) => ...
(or false true) false true => ...
(true true false) false true => ...
true false true => ...
false
```

¬(TRUE ⋁ FALSE) ≡ FALSE

```
λx.λy(not (or x y)) true false => ...
not (or true false) => ...
(or true false) false true => ...
(false true true) false true => ...
true false true => ...
false
```

¬(TRUE ⋁ TRUE) ≡ FALSE

```
λx.λy(not (or x y)) true true => ...
not (or true true) => ...
(or true true) false true => ...
(true true true) false true => ...
true false true => ...
false
```

##### (b) p → q ≡ ¬q → ¬p

¬FALSE → ¬FALSE ≡ TRUE

```
λp.λq.(implies (not q) (not p)) false false => ...
implies (not false) (not false) => ...
(not false) (not false) true => ...
true (not false) true => ...
not false => ...
true
```

¬FALSE → ¬TRUE ≡ TRUE

```
λp.λq.(implies (not q) (not p)) false true => ...
implies (not true) (not false) => ...
(not true) (not false) true => ...
false (not false) true => ...
true
```

¬TRUE → ¬FALSE ≡ FALSE

```
λp.λq.(implies (not q) (not p)) true false => ...
implies (not false) (not true) => ...
(not false) (not true) true => ...
true (not true)  true => ...
not true => ...
false
```

¬TRUE → ¬TRUE ≡ TRUE

```
λp.λq.(implies (not q) (not p)) true true => ...
implies (not true) (not true) => ...
(not true) (not true) true => ...
false (not true) true => ...
true
```

##### (c) ¬p ≡ ¬(¬(¬p))

¬(¬(¬FALSE)) ≡ TRUE

```
λp.(not (not (not p))) false => ...
not (not (not false)) => ...
not (not true) => ...
not false => ...
true
```

¬(¬(¬TRUE)) ≡ FALSE

```
λp.(not (not (not p))) true => ...
not (not (not true)) => ...
not (not false) => ...
not true => ...
false
```

##### (d) p → q ≡ ¬(p ∧ ¬q)

¬(FALSE ∧ ¬FALSE) ≡ TRUE

```
λp.λq.(not (and p (not q))) false false => ...
not (and false (not false)) => ...
(and false (not false)) false true => ...
(false (not false) false) false true => ...
false false true => ...
true
```

¬(FALSE ∧ ¬TRUE) ≡ TRUE

```
λp.λq.(not (and p (not q))) false true => ...
not (and false (not true)) => ...
(and false (not true)) false true => ...
(false (not true) false) false true => ...
false false true => ...
true
```

¬(TRUE ∧ ¬FALSE) ≡ FALSE

```
λp.λq.(not (and p (not q))) true false => ...
not (and true (not false)) => ...
(and true (not false)) false true => ...
(true (not false) false) false true => ...
(not false) false true => ...
true false true => ...
false
```

¬(TRUE ∧ ¬TRUE) ≡ TRUE

```
λp.λq.(not (and p (not q))) true true => ...
not (and true (not true)) => ...
(and true (not true)) false true => ...
(true (not true) false) false true => ...
(not true) false true => ...
false false true => ...
true
```

##### (e) p ↔ q ≡ (p → q) ∧ (q → p)

(FALSE → FALSE) ∧ (FALSE → FALSE) ≡ TRUE

```
λp.λq.(and (implies p q) (implies q p)) false false => ...
and (implies false false) (implies false false) => ...
(implies false false) (implies false false) false => ...
true (implies false false) false => ...
implies false false => ...
true
```

(FALSE → TRUE) ∧ (TRUE → FALSE) ≡ FALSE

```
λp.λq.(and (implies p q) (implies q p)) false true => ...
and (implies false true) (implies true false) => ...
(implies false true) (implies true false) false => ...
true (implies true false) false => ...
implies true false => ...
false
```

(TRUE → FALSE) ∧ (FALSE → TRUE) ≡ FALSE

```
λp.λq.(and (implies p q) (implies q p)) true false => ...
and (implies true false) (implies false true) => ...
(implies true false) (implies false true) false => ...
false (implies false true) false => ...
false
```

(TRUE → TRUE) ∧ (TRUE → TRUE) ≡ TRUE

```
λp.λq.(and (implies p q) (implies q p)) true true => ...
and (implies true true) (implies true true) => ...
(implies true true) (implies true true) false => ...
true (implies true true) false => ...
implies true true => ...
true
```

#### 3.4: show that λx.(succ (pred x)) and λx.(pred (succ x))

are equivalent for any non-zero arg

```
λx.(succ (pred x)) λs.((s false) <number>) => ...
succ (pred λs.((s false) <number>)) => ...
succ <number> => ...
λs.((s false) <number>)
```

```
λx.(pred (succ x)) λs.((s false) <number>) => ...
pred (succ λs.((s false) <number>)) => ...
pred λs.((s false) λs.((s false) <number>)) ==
λn.(((is_zero n) zero) (n select_second)) λs.((s false) λs.((s false) <number>)) => ...
λs.((s false) λs.((s false) <number>)) select_second => ...
select_second false λs.((s false) <number>) => ...
λs.((s false) <number>)
```

are not equivalent for zero arg

```
λx.(succ (pred x)) zero => ...
succ (pred zero) => ...
succ zero ==
one
```

```
λx.(pred (succ x)) zero => ...
pred (succ zero) => ...
pred one => ...
zero
```

#### XOR

| p | q | p ⊕ q |
| - | - | :---: |
| F | F |   F   |
| F | T |   T   |
| T | F |   T   |
| T | T |   F   |

```
def xor = 
```