### Recursive function constructor

```
def recursive f = λs.(f (s s)) λs.(f (s s))
```

### Addition

```
def add_aux f x y =
    if is_zero y
    then x
    else (f (succ x) (pred y))

def add = recursive add_aux
```

```
add one two ==
(λf.(λs.(f (s s)) λs.(f (s s))) add_aux) one two =>
(λs.(add_aux (s s)) λs.(add_aux (s s))) one two =>
(add_aux (λs.(add_aux (s s)) λs.(add_aux (s s)))) one two ==
(λf.λx.λy.
    if is_zero y
    then x
    else (f (succ x) (pred y)) (λs.(add_aux (s s)) λs.(add_aux (s s)))) one two =>
λx.λy.
    if is_zero y
    then x
    else ((λs.(add_aux (s s)) λs.(add_aux (s s))) (succ x) (pred y)) one two => ... =>
if is_zero two
then one
else ((λs.(add_aux (s s)) λs.(add_aux (s s))) (succ one) (pred two)) => ... =>
((add_aux (λs.(add_aux (s s)) λs.(add_aux (s s)))) (succ one) (pred two)) ==
((λf.λx.λy.
    if is_zero y
    then x
    else (f (succ x) (pred y)) (λs.(add_aux (s s)) λs.(add_aux (s s)))) (succ one) (pred two)) => ... =>
if is_zero (pred two)
then (succ one)
else ((λs.(add_aux (s s)) λs.(add_aux (s s))) (succ (succ one)) (pred (pred two))) => ... =>
((add_aux (λs.(add_aux (s s)) λs.(add_aux (s s)))) (succ (succ one)) (pred (pred two))) ==
((λf.λx.λy.
    if is_zero y
    then x
    else (f (succ x) (pred y)) (λs.(add_aux (s s)) λs.(add_aux (s s)))) (succ (succ one)) (pred (pred two))) =>
(λx.λy.
    if is_zero y
    then x
    else ((λs.(add_aux (s s)) λs.(add_aux (s s))) (succ x) (pred y)) (succ (succ one)) (pred (pred two))) => ... =>
if is_zero (pred (pred two))
    then (succ (succ one))
    else ((λs.(add_aux (s s)) λs.(add_aux (s s))) (succ (succ (succ one))) (pred (pred (pred two)))) => ... =>
(succ (succ one)) ==
three
```

### Recursive notation: paradoxical combinator Y

```
rec <name> = <expression>
```

is replaced by:

```
def <name1> f = ... (f f ...) ...
def <name> = recursive <name1>
```

### Arithmetics operations

```
rec add x y =
    if is_zero y
    then x
    else add (succ x) (pred y)
```

```
rec mult x y =
    if is_zero y
    then zero
    else add x (mult x (pred y))
```

```
rec power x y =
    if is_zero y
    then one
    else mult x (power x (pred y))
```

```
rec sub x y =
    if is_zero y
    return x
    else sub (pred x) (pred y)
```

```
def abs_diff x y = add (sub x y) (sub y x)
```

```
def equal x y = is_zero (abs_diff x y)
```

```
def greater x y = not (is_zero (sub x y))
```

```
def greater_or_equal x y = is_zero (sub y x)
```

```
def less_or_equal x y = greater_or_equal y x
```

```
rec div x y =
    if is_zero y
    then zero
    else if greater y x
            then zero
            else succ (div (sub x y) y)
```

### 4.2 evaluate expression

```
def sum1 f n =
    if is_zero n
    then zero
    else add n (f (pred n))

def sum = recursive sum1

sum three ==
recursive sum1 three ==
λf.(λs.(f (s s)) λs.(f (s s))) sum1 three =>
(sum1 (λs.(sum1 (s s)) λs.(sum1 (s s)))) three ==
(λf.λn.if is_zero n
    then zero
    else add n (f (pred n)) (λs.(sum1 (s s)) λs.(sum1 (s s)))) three =>
λn.if is_zero n
    then zero
    else add n ((λs.(sum1 (s s)) λs.(sum1 (s s))) (pred n)) three =>
if is_zero three
    then zero
    else add three ((λs.(sum1 (s s)) λs.(sum1 (s s))) (pred three)) -> ... ->
add three (add two ((λs.(sum1 (s s)) λs.(sum1 (s s))) (pred two))) -> ... ->
add three (add two (add one ((λs.(sum1 (s s)) λs.(sum1 (s s))) (pred one)))) -> ... ->
add three (add two (add one zero)) -> ... ->
six
```

### 4.2 factorial function

```
def prod1 f n =
    if less_or_equal one
    then one
    else mult n (f (pred n))

def prod = recursive prod1

prod three ==
recursive prod1 three => ... =>
prod1 (recursive prod1) three => ... =>
mult three ((recursive prod1) (pred three)) -> ... ->
mult three (prod1 (recursive prod1) two) -> ... ->
mult three (mult two ((recursive prod1) (pred two))) -> ... ->
mult three (mult two (prod1 (recursive prod1) one)) -> ... ->
mult three (mult two one) -> ... ->
mult three two -> ... ->
six
```

### 4.3 sum by function

```
def fun_sum1 f fun n =
    if is_zero n
    then fun zero
    else add (fun n) (f fun (pred n))

def fun_sum = recursive fun_sum1

def dobule = x = add x x

fun_sum double three ==
recursive fun_sum1 double three => ... =>
fun_sum1 (recursive fun_sum1) double three => ... =>
add (double three) ((recursive fun_sum1) double (pred three)) -> ... ->
add six (fun_sum1 (recursive fun_sum1) double two) -> ... ->
add six (add four (fun_sum1 (recursive fun_sum1) double one)) -> ... ->
add six (add four (add two (fun_sum1 (recursive fun_sum1) double zero))) -> ... ->
add six (add four (add two (double zero))) -> ... ->
twelve
```

### 4.4 sum by function with step

```
def fun_sum_step1 f fun n s =
    if is_zero n
    then fun n
    else add (fun n) (f fun (sub n s) s)

def fun_sum_step = recursive fun_sum_step1

fun_sum_step dobule five two ==
recursive fun_sum_step1 dobule five two => ... =>
fun_sum_step1 (recursive fun_sum_step1) dobule five two => ... =>
add (dobule five) ((recursive fun_sum_step1) dobule (sub five two) two) -> ... ->
add ten (fun_sum_step1 (recursive fun_sum_step1) dobule three two) -> ... ->
add ten (add six (recursive (recursive fun_sum_step1) dobule one two)) -> ...->
add ten (add six (add two (recursive (recursive fun_sum_step1) dobule zero two))) -> ... ->
add ten (add six (add two (dobule zero))) -> ... ->
eighteen

fun_sum_step dobule four two ==
recursive fun_sum_step1 dobule four two => ... =>
fun_sum_step1 (recursive fun_sum_step1) dobule four two => ... =>
add eight (fun_sum_step1 (recursive fun_sum_step1) dobule two two) -> ... ->
add eight (add four (recursive (recursive fun_sum_step1) dobule zero two)) -> ... ->
add eight (add four ((dobule zero))) -> ... ->
twelve
```